platform/tests/Echo.v
@@ -1,25 +1,51 @@
-Require Import AutoSep.
+Require Import AutoSep Malloc Arrays8.
 
 
-Definition mainS := SPEC reserving 4
-  PREonly[_] Emp.
+Definition mainS := SPEC reserving 12
+  PREonly[_] mallocHeap 0.
+
+Opaque allocated.
 
 Definition m := bimport [[ "sys"!"abort" @ [abortS], "sys"!"printInt" @ [printIntS],
                            "sys"!"listen" @ [listenS], "sys"!"accept" @ [acceptS],
-                           "sys"!"read" @ [readS], "sys"!"write" @ [writeS] ]]
+                           "sys"!"read" @ [readS], "sys"!"write" @ [writeS],
+                           "malloc"!"malloc" @ [mallocS] ]]
   bmodule "test" {{
-    bfunctionNoRet "main"("fdl", "fd") [mainS]
+    bfunctionNoRet "main"("fdl", "fd", "buf", "n") [mainS]
       "fdl" <-- Call "sys"!"listen"(8080%N)
-      [PREonly[_] Emp];;
+      [PREonly[_] mallocHeap 0];;
 
       "fd" <-- Call "sys"!"accept"("fdl")
-      [PREonly[_] Emp];;
+      [PREonly[_] mallocHeap 0];;
+
+      "buf" <-- Call "malloc"!"malloc"(0, 10)
+      [PREonly[_, R] R =?> 10];;
+
+      Note [please_materialize_buffer 10];;
+
+      "n" <-- Call "sys"!"read"("fd", "buf", 40)
+      [PREonly[V] V "buf" =?>8 40];;
+
+      [PREonly[V] V "buf" =?>8 40]
+      While ("n" <> 0) {
+        Call "sys"!"printInt"("n")
+        [PREonly[V] V "buf" =?>8 40];;
+
+        "n" <-- Call "sys"!"read"("fd", "buf", 40)
+        [PREonly[V] V "buf" =?>8 40]
+      };;
 
       Call "sys"!"abort"()
       [PREonly[_] [| False |] ]
     end
   }}.
 
+Definition hints : TacPackage.
+  prepare materialize_buffer tt.
+Defined.
+
+Ltac t := solve [ sep hints; auto ].
+
 Theorem ok : moduleOk m.
-  vcgen; abstract sep_auto.
+  vcgen; abstract (sep hints; auto).
 Qed.
